---
title: "Hyperbole"
---
## Formula

$\Huge{\frac{(x-h)^2}{a^2} - \frac{(y-k)^2}{b^2} = 1}$  (horizontal hyperbole)

$\Huge{\frac{(y-k)^2}{a^2} - \frac{(x-h)^2}{b^2} = 1}$ (vertical hyperbole)

**Reminder: go opposite way of the values in the brackets**

c$^2$ = a$^2$ + b$^2$ 
c represents the focus
a represents the vertex (up / down a or left right a depending on which type of hyperbola)

## Horizontal Hyperbole

asymptote: $\frac{b}{a}$ & -$\frac{b}{a}$
asymptote:  y - k = $\pm$ $\frac{b}{a}$(x-h) 
e (eccentricity) = $\frac{c}{a}$
e > 1

the vertex is a units left a units right from origin

![[images/IMG_2434.jpg]]

## Vertical Hyperbole

asymptote:
y - k = $\pm$ $\frac{a}{b}$ (x-h)
e (eccentricity) = $\frac{c}{a}$
e > 1

the vertex is a units up and a units down from origin
focus is c units up and c units down
b value is to the right and left and if you connect all the points it creates a box
